hol/cake_export/p4_exec_sem_vss_cakeProgScript.sml
@@ -64,60 +64,7 @@ Definition vss_copyout_pbl'_def:
     | NONE => NONE)
   | _ => NONE
 End
-
-Definition vss_packet_in_extract_gen_def:
- (vss_packet_in_extract_gen ascope_lookup (ascope_update:num #
-    (num # (core_v_ext + vss_v_ext)) list #
-    (string # p4$v) list #
-    (string # (((e list -> bool) # num) # string # e list) list) list ->
-    num ->
-    core_v_ext + vss_v_ext ->
-    num #
-    (num # (core_v_ext + vss_v_ext)) list #
-    (string # p4$v) list #
-    (string # (((e list -> bool) # num) # string # e list) list) list) ascope_update_v_map (ascope:vss_ascope, g_scope_list:g_scope_list, scope_list) =
-  case lookup_lval' scope_list (lval_varname (varn_name "this")) of
-  | SOME (v_ext_ref i) =>
-   (case lookup_lval_header scope_list (lval_varname (varn_name "headerLvalue")) of
-    | SOME (valid_bit, x_v_l) =>
-     (case lookup_ascope_gen ascope_lookup ascope i of
-      | SOME ((INL (core_v_ext_packet packet_in_bl)):(core_v_ext, vss_v_ext) sum) =>
-       (case size_in_bits (v_header valid_bit x_v_l) of
-        | SOME size' =>
-         if arithmetic$<= size' (LENGTH packet_in_bl)
-         then
-          (case set_header x_v_l packet_in_bl of
-           | SOME header =>
-            (case assign' scope_list header (lval_varname (varn_name "headerLvalue")) of
-             | SOME scope_list' =>
-              SOME (update_ascope_gen ascope_update ascope i ((INL (core_v_ext_packet (DROP size' packet_in_bl))):(core_v_ext, vss_v_ext) sum), scope_list', status_returnv v_bot)
-             | NONE => NONE)
-           | NONE => NONE)
-         else
-          (* NOTE: Specific serialisation of errors is assumed here - "PacketTooShort" -> 1 *)
-          SOME (ascope_update_v_map (update_ascope_gen ascope_update ascope i ((INL (core_v_ext_packet [])):(core_v_ext, vss_v_ext) sum)) "parseError" (v_bit (fixwidth 32 (n2v 1), 32)), scope_list, status_trans "reject")
-        | NONE => NONE)
-       | _ => NONE)
-    | NONE => NONE)
-  | _ => NONE
- )
-End
-
-(* TODO: Why do we need to fix the packet_in_extract stuff? *)
-Definition vss_packet_in_extract'_def:
- vss_packet_in_extract':((num #
-  (num # (core_v_ext + vss_v_ext)) list #
-  (string # p4$v) list #
-  (string # (((e list -> bool) # num) # string # e list) list) list) #
- (varn # p4$v # lval option) list list #
- (varn # p4$v # lval option) list list ->
- ((num #
-   (num # (core_v_ext + vss_v_ext)) list #
-   (string # p4$v) list #
-   (string # (((e list -> bool) # num) # string # e list) list) list) #
-  (varn # p4$v # lval option) list list # status) option) = vss_packet_in_extract_gen vss_ascope_lookup vss_ascope_update vss_ascope_update_v_map
-End
-
+(*
 Definition Checksum16_construct'_def:
  (Checksum16_construct' ((counter, ext_obj_map, v_map, ctrl):vss_ascope, g_scope_list:g_scope_list, scope_list) =
   let ext_obj_map' = p4$AUPDATE ext_obj_map (counter, INR (vss_v_ext_ipv4_checksum ([]:(bool list) list))) in
@@ -185,55 +132,11 @@ Definition Checksum16_get'_def:
   | _ => NONE
  )
 End
-
-fun mk_v_bitii' (num, width) =
- let
-  val width_tm = numSyntax.term_of_int width
- in
-  mk_v_bit $ pairSyntax.mk_pair (bitstringSyntax.mk_fixwidth (width_tm, bitstringSyntax.mk_n2v $ numSyntax.term_of_int num), width_tm)
- end
-;
-
-(*
-(* TODO: Hack, some type mismatch when using regular syntax functions *)
-val (v_header_tm, mk_v_header, dest_v_header, is_v_header) =
-  syntax_fns2 "p4" "v_header";
-fun mk_v_header_list vbit x_v_l =
-  mk_v_header (vbit, (listSyntax.mk_list ((map (fn (a, b) => mk_pair (a, b)) x_v_l), ``:(string # p4$v) ``)));
-val (v_struct_tm, mk_v_struct, dest_v_struct, is_v_struct) =
-  syntax_fns1 "p4" "v_struct";
-fun mk_v_struct_list x_v_l =
-  mk_v_struct (listSyntax.mk_list ((map (fn (a, b) => mk_pair (a, b)) x_v_l), ``:(string # p4$v)``));
-
-val ipv4_header_uninit =
- mk_v_header_list F 
-                  [(``"version"``, mk_v_bitii' (0, 4)),
-                   (``"ihl"``, mk_v_bitii' (0, 4)),
-                   (``"diffserv"``, mk_v_bitii' (0, 8)),
-                   (``"totalLen"``, mk_v_bitii' (0, 16)),
-                   (``"identification"``, mk_v_bitii' (0, 16)),
-                   (``"flags"``, mk_v_bitii' (0, 3)),
-                   (``"fragOffset"``, mk_v_bitii' (0, 13)),
-                   (``"ttl"``, mk_v_bitii' (0, 8)),
-                   (``"protocol"``, mk_v_bitii' (0, 8)),
-                   (``"hdrChecksum"``, mk_v_bitii' (0, 16)),
-                   (``"srcAddr"``, mk_v_bitii' (0, 32)),
-                   (``"dstAddr"``, mk_v_bitii' (0, 32))];
-val ethernet_header_uninit =
- mk_v_header_list F
-                  [(``"dstAddr"``, mk_v_bitii' (0, 48)),
-                   (``"srcAddr"``, mk_v_bitii' (0, 48)),
-                   (``"etherType"``, mk_v_bitii' (0, 16))];
-val vss_parsed_packet_struct_uninit =
- mk_v_struct_list [(``"ethernet"``, ethernet_header_uninit), (``"ip"``, ipv4_header_uninit)];
 *)
-
 
 val _ = translation_extends "p4_exec_sem_arch_cakeProg";
 
 val _ = ml_prog_update (open_module "p4_exec_sem_vss_cake");
-
-val _ = translate arch_multi_exec'_def;
 
 val _ = translate vss_parser_runtime_def;
 
@@ -259,34 +162,34 @@ val _ = translate vss_ascope_update_v_map_def;
 val _ = translate verify_gen_def;
 val _ = translate vss_verify;
 
-val _ = translate Checksum16_construct'_def;
+val _ = translate Checksum16_construct_def;
 
-val _ = translate Checksum16_clear'_def;
+val _ = translate Checksum16_clear_def;
 
 val _ = translate oTAKE_DROP_def;
 val _ = translate v2w16s'''_def;
 val _ = translate header_entries2v_def;
 val _ = translate v2w16s''_def;
 val _ = translate get_checksum_incr''_def;
-val _ = translate Checksum16_update'_def;
+val _ = translate Checksum16_update_def;
 
 val _ = translate add_with_carry'_def;
 val _ = translate add_ones_complement'_def;
-val _ = translate compute_checksum16'_inner_def;
+val _ = translate compute_checksum16_inner_def;
 val _ = translate all_lists_length_16_def;
-val _ = translate compute_checksum16'_def;
-Theorem compute_checksum16'_side:
-!v1. compute_checksum16'_side v1
+val _ = translate compute_checksum16_def;
+Theorem compute_checksum16_side:
+!v1. compute_checksum16_side v1
 Proof
-simp[Once $ definition "compute_checksum16'_side_def"] \\
+simp[Once $ definition "compute_checksum16_side_def"] \\
 Induct >- (
- simp[Once $ theorem "compute_checksum16'_inner_side_def", all_lists_length_16_def]
+ simp[Once $ theorem "compute_checksum16_inner_side_def", all_lists_length_16_def]
 ) \\
 rpt strip_tac \\
-gs[all_lists_length_16_def, Once $ theorem "compute_checksum16'_inner_side_def"] \\
+gs[all_lists_length_16_def, Once $ theorem "compute_checksum16_inner_side_def"] \\
 Cases_on ‘v1’ >- (
- gs[theorem "compute_checksum16'_inner_side_def",
-    compute_checksum16'_inner_def, Once $ definition "add_ones_complement'_side_def",
+ gs[theorem "compute_checksum16_inner_side_def",
+    compute_checksum16_inner_def, Once $ definition "add_ones_complement'_side_def",
     Once $ definition "add_with_carry'_side_def"] \\
  rpt strip_tac \\ (
   gs[bitstringTheory.fixwidth_def, AllCaseEqs(), bitstringTheory.zero_extend_def,
@@ -294,23 +197,26 @@ Cases_on ‘v1’ >- (
  ) 
 ) \\
 qpat_x_assum ‘!x2 x1. _’ (fn thm => ASSUME_TAC $ Q.SPECL [‘h'’, ‘t’] thm) \\
-simp[Once $ theorem "compute_checksum16'_inner_side_def",
+simp[Once $ theorem "compute_checksum16_inner_side_def",
      Once $ definition "add_ones_complement'_side_def",
      Once $ definition "add_with_carry'_side_def"] \\
 rpt strip_tac >- (
  gs[]
 ) >- (
- gs[compute_checksum16'_inner_def, add_ones_complement'_def, add_with_carry'_def, AllCaseEqs(), bitstringTheory.fixwidth_def, AllCaseEqs(), bitstringTheory.zero_extend_def, listTheory.PAD_LEFT]
+ gs[compute_checksum16_inner_def, add_ones_complement'_def, add_with_carry'_def,
+    AllCaseEqs(), bitstringTheory.fixwidth_def, AllCaseEqs(),
+    bitstringTheory.zero_extend_def, listTheory.PAD_LEFT]
 ) >- (
  gs[]
 ) >- (
- gs[bitstringTheory.fixwidth_def, AllCaseEqs(), bitstringTheory.zero_extend_def, listTheory.PAD_LEFT]
+ gs[bitstringTheory.fixwidth_def, AllCaseEqs(), bitstringTheory.zero_extend_def,
+    listTheory.PAD_LEFT]
 ) \\
-simp[Once $ theorem "compute_checksum16'_inner_side_def"]
+simp[Once $ theorem "compute_checksum16_inner_side_def"]
 QED
-val _ = update_precondition compute_checksum16'_side;
-val _ = translate ALOOKUP_compute_checksum16'_def;
-val _ = translate Checksum16_get'_def;
+val _ = update_precondition compute_checksum16_side;
+val _ = translate ALOOKUP_compute_checksum16_def;
+val _ = translate Checksum16_get_def;
 
 val _ = translate vss_ascope_update_def;
 val _ = translate vss_ascope_lookup_def;
@@ -321,13 +227,12 @@ val _ = translate set_bool_def;
 val _ = translate size_in_bits_def;
 val _ = translate set_fields_def;
 val _ = translate set_header_def;
-
 val _ = translate lookup_ascope_gen_def;
-val _ = translate lookup_lval_header_def;
+val _ = translate p4_coreTheory.lookup_lval_header_def;
 val _ = translate packet_in_extract_gen_def;
-val _ = translate vss_packet_in_extract_gen_def;
-val _ = translate vss_packet_in_extract'_def;
-
+val _ = translate vss_ascope_update_v_map_def;
+val _ = translate vss_packet_in_extract;
+        
 val _ = translate flatten_v_l_def;
 val _ = translate packet_out_emit_gen_def;
 val _ = translate vss_packet_out_emit;
